Three dimensional positioning 
=============================

Both horizontal and vertical components have been explained and now can be combined into one system. To implement a three dimensional system, we simply need to replace our #b_n# variable in the vertical plane equation with the horizontal plane equations. The result is:
## a_1(x,y,z) = \sqrt{( {\sqrt{3}\over 3} D - y + r)^2 + x^2} + z##
## a_2(x,y,z) = \sqrt{ ({1\over 2} D + x - {1\over 2} r )^2 + ({\sqrt{3}\over 6} D + y - {\sqrt{3}\over 2}r )^2 } + z##
## a_3(x,y,z) =  \sqrt{ ({1\over 2} D - x + {1\over 2} r )^2 + ({\sqrt{3}\over 6} D + y - {\sqrt{3}\over 2}r  )^2 } + z##
